feat(*) cleanup before submission

Examples/E_Unification_Examples.thy
@@ -13,6 +13,7 @@ text \<open>Sample applications of e-unifiers, methods, etc. introduced in this 
 experiment
 begin
 
+
 paragraph \<open>Using the simplifier for unification.\<close>
 
 inductive_set even :: "nat set" where
@@ -23,20 +24,24 @@ text \<open>Premises of the form @{term "SIMPS_TO_UNIF lhs rhs"} are solved by
 @{ML_structure Simplifier_Unification}. It first normalises @{term lhs} and then unifies the
 normalisation with @{term rhs}. See also @{theory ML_Unification.ML_Unification_HOL_Setup}.\<close>
 
-lemma [unif_hint]: "n \<noteq> 0 \<Longrightarrow> PROP SIMPS_TO_UNIF (n - 1) m \<Longrightarrow> n \<equiv> Suc m"
+lemma [unif_hint where prio = Prio.LOW]: "n \<noteq> 0 \<Longrightarrow> PROP SIMPS_TO_UNIF (n - 1) m \<Longrightarrow> n \<equiv> Suc m"
   unfolding SIMPS_TO_UNIF_eq by linarith
 
-schematic_goal "(\<And>x. x + 2 = n) \<Longrightarrow> Suc ?x = n"
+text \<open>By default, below unification methods use
+@{ML Standard_Mixed_Unification.first_higherp_first_comb_higher_unify}, which is a combination of
+various practical unification algorithms.\<close>
+
+schematic_goal "(\<And>x. x + 4 = n) \<Longrightarrow> Suc ?x = n"
   by uassm
 
-schematic_goal "6 \<in> even"
+lemma "6 \<in> even"
   apply (urule step)
   apply (urule step)
   apply (urule step)
   apply (urule zero)
   done
 
-schematic_goal "(220 + (80 - 2 * 2)) \<in> even"
+lemma "(220 + (80 - 2 * 2)) \<in> even"
   apply (urule step)
   apply (urule step)+
   apply (urule zero)
@@ -47,10 +52,12 @@ lemma
   shows "[a] @ [b,c] = [c,b,a]"
   using assms by uassm
 
-lemma "(x + (y :: nat))^2 \<le> x^2 + 2*x*y + y^2"
-  supply power2_sum[simp]
-  by (ufact order.refl)
+lemma "x \<in> ({z, y, x} \<union> S) \<inter> {x}"
+  by (ufact TrueI)
 
+lemma "(x + (y :: nat))^2 \<le> x^2 + 2*x*y + y^2 + 4 * y + x - y"
+  supply power2_sum[simp]
+  by (ufact TrueI)
 
 paragraph \<open>Providing canonical solutions for meta variables with unification hints\<close>
 
@@ -59,13 +66,58 @@ lemma [unif_hint]: "xs \<equiv> [] \<Longrightarrow> length xs \<equiv> 0" by si
 schematic_goal "length ?xs = 0"
   by (ufact refl)
 
+lemma [unif_hint]: "(n :: nat) \<equiv> m \<Longrightarrow> n - m \<equiv> 0" by simp
+
+schematic_goal "n - ?m = (0 :: nat)"
+  by (ufact refl)
+
+text \<open>The following fails because, by default, @{ML Standard_Unification_Hints.try_hints}
+uses the higher-order pattern unifier to unify hints against a given disagreement pair, and
+@{term 0} cannot be higher-order pattern unified with @{term "length []"}. The unification of the
+hint requires the use of yet another hint, namely @{term "length xs = 0"} (cf. above).\<close>
+schematic_goal "n - ?m = length []"
+  \<comment> \<open>by (ufact refl)\<close>
+  oops
+
+text \<open>There are two ways to fix this:
+\<^enum> We allow the recursive uses of unification hints when searching for suitable unification hints.
+\<^enum> We use a different unification hint that the recursive use of hints explicit.\<close>
+
+text \<open>Solution 1: recursive usages of hints. Warning: such recursive applications easily loop.\<close>
+schematic_goal "n - ?m = length []"
+  using [[unif_hint where concl_unifier = Standard_Mixed_Unification.first_higherp_first_comb_higher_unify]]
+  by (ufact refl)
+
+text \<open>Solution 2: make the recursion explicit in the hint.\<close>
+
+lemma [unif_hint]: "k \<equiv> 0 \<Longrightarrow> (n :: nat) \<equiv> m \<Longrightarrow> n - m \<equiv> k" by simp
+
+schematic_goal "n - ?m = length []"
+  by (ufact refl)
+
 
 paragraph \<open>Strenghten unification with unification hints\<close>
+
+lemma
+  assumes [unif_hint]: "n = m"
+  shows "n - m = (0 :: nat)"
+  by (ufact refl)
 
 lemma
   assumes "x = y"
   shows "y = x"
   supply eq_commute[unif_hint]
+  by (ufact assms)
+
+
+text \<open>Unfolding definitions.\<close>
+
+definition "mysuc n = Suc n"
+
+lemma
+  assumes "\<And>m. Suc n > mysuc m"
+  shows "mysuc n > Suc 3"
+  supply mysuc_def[unif_hint]
   by (ufact assms)
 
 
@@ -79,6 +131,19 @@ lemma
   assumes "A \<longrightarrow> (B \<longrightarrow> C) \<longrightarrow> D"
   shows "A \<Longrightarrow> (B \<Longrightarrow> C) \<Longrightarrow> D"
   using assms by ufact
+
+
+paragraph \<open>Better control over meta variable instantiations\<close>
+
+text \<open>Consider the following type-inference problem.\<close>
+schematic_goal
+  assumes app_typeI: "\<And>f x.  (\<And>x. ArgT x \<Longrightarrow> DomT x (f x)) \<Longrightarrow> ArgT x \<Longrightarrow> DomT x (f x)"
+  and f_type: "\<And>x. ArgT x \<Longrightarrow> DomT x (f x)"
+  and x_type: "ArgT x"
+  shows "?T (f x)"
+  apply (urule app_typeI) \<comment>\<open>compare with the following application, creating an unintuitive instantiation\<close>
+  (* apply (rule app_typeI) *)
+  oops
 
 end
 
