Unification_Hints/ML_Unification_Hints.thy
@@ -30,10 +30,9 @@ ML\<open>
     and more_args = \<open>
       structure TI = Discrimination_Tree
       val init_args = {
-        concl_unifier = SOME Higher_Order_Pattern_Unification.unify,
-        normalisers = SOME (Standard_Mixed_Unification.norm_term_first_higherp_comb_higher_unify,
-          Standard_Mixed_Unification.norm_thm_first_higherp_comb_higher_unify),
-        prems_unifier = SOME (Standard_Mixed_Unification.first_higherp_comb_higher_unify
+        concl_unifier = SOME Higher_Ordern_Pattern_First_Decomp_Unification.unify,
+        normalisers = SOME Standard_Mixed_Unification.norms_first_higherp_first_comb_higher_unify,
+        prems_unifier = SOME (Standard_Mixed_Unification.first_higherp_first_comb_higher_unify
           |> Unification_Combinator.norm_unifier Envir_Normalisation.beta_norm_term_unif),
         retrieval = SOME (Term_Index_Unification_Hints_Args.mk_sym_retrieval
           TI.norm_term TI.unifiables),
@@ -47,7 +46,7 @@ text\<open>Standard unification hints are accessible via @{attribute unif_hint}.
 declare [[ucombine add = \<open>Standard_Unification_Combine.eunif_data
   (Standard_Unification_Hints.try_hints
   |> Unification_Combinator.norm_unifier
-    Standard_Mixed_Unification.norm_term_first_higherp_comb_higher_unify
+    (#norm_term Standard_Mixed_Unification.norms_first_higherp_first_comb_higher_unify)
   |> K)
   (Standard_Unification_Combine.default_metadata Standard_Unification_Hints.binding)\<close>]]
 
